WIP on the proof of the stack machine

examples/Stack.v
@@ -1,25 +1,188 @@
-Require Import Common. 
+Require Import Common Arith Peano. 
 Open Scope Z_scope. 
 
 Require Import Core Front. 
-
 (** 
 
 In this file, we define a hardware implementation of a small subset of
 the Java Virtual Machine. We take the following conventions: 
 
 - the size of the code, the size of the stack, and the number of
-registers are the same. 
+  registers are the same.
 
 - the state of the machine is defined by a program counter, that
   denotes the position in the code; a stack pointer, that denotes the
-  first free element above the stack; and a set of registers. 
+  first free element above the stack; and a set of registers.
 
 *)
 
+
+Definition Next {A} (f : A -> option A) (m : A ):= 
+  match f m with 
+    | None => m
+    | Some m => m
+  end. 
+
+Module Spec. 
+
+  Notation id := nat. 
+  Inductive cond := Ceq | Cne | Cle | Cgt. 
+  Inductive instruction: Type :=
+  | Iconst(n: nat) 
+  | Ivar(x: id)
+  | Isetvar(x: id) 
+  | Iadd 
+  | Isub 
+  | Ibranch_forward(ofs: nat)
+  | Ibranch_backward(ofs: nat)
+  | Ibranch_cond (c : cond) (ofs : nat)
+  | Ihalt. 
+
+  
+  Definition code := list instruction.
+
+
+  Fixpoint code_at (C: code) (pc: nat) : option instruction :=
+    match C, pc with
+      | nil, _ => None
+      | i :: C', O => Some i
+      | i :: C', S pc' => code_at C' pc'
+    end%list.
+  
+  Definition stack := list nat.
+  
+  Definition store := id -> nat. 
+
+  Require Import NPeano. 
+
+  Definition update (s:store) (x:id) (v : nat) := 
+    fun y => if Nat.eqb x y then v else s y.
+  
+  Record machine := mk
+    {
+      c   : code;      
+      pc : nat;
+      stk : stack;
+      str : store
+    }.
+  
+  Require Import List. 
+  
+  Section t. 
+    (** Dynamic check that the state we reach is valid  *)
+  
+    Variable max_pc : nat.
+    Definition dyncheck  (s : machine) :=
+      if Nat.ltb (pc s) max_pc then 
+        Some s
+      else None.
+    
+    Definition step (s : machine) : option machine :=
+      do op <- code_at (c s) (pc s);
+      match op with 
+        | Iconst n => dyncheck (mk (c s) (pc s +1) (n :: stk s) (str s))
+        | Ivar x =>   dyncheck (mk (c s) (pc s +1) ((str s) x :: stk s) (str s))
+        | Isetvar x => 
+          match stk s with
+            | nil => None
+            | v :: stk => 
+              dyncheck (mk (c s) (pc s +1) (stk) (update (str s) x v))
+          end
+        | Iadd =>
+          match stk s with
+            | nil => None
+            | cons _ nil => None
+            | n1 :: n2 :: stk => 
+              dyncheck (mk (c s) (pc s +1) (n1 + n2 :: stk)  (str s) )
+          end
+        | Isub =>
+          match stk s with
+            | nil => None
+            | cons _ nil => None
+            | n2 :: n1 :: stk => 
+              dyncheck (mk (c s) (pc s +1) (n1 - n2 :: stk)  (str s) )
+          end
+        | Ibranch_forward ofs => 
+          dyncheck (mk (c s) (pc s + 1 + ofs) (stk s) (str s))
+        | Ibranch_backward ofs => 
+          check (ofs <=? pc s + 1);
+          dyncheck (mk (c s) (pc s + 1 - ofs) (stk s) (str s))
+        | Ibranch_cond test ofs => 
+          match stk s with
+            | nil => None
+            | cons _ nil => None
+            | n2 :: n1 :: stk => 
+              let t := match test with 
+                           | Ceq => NPeano.Nat.eqb n1 n2 
+                           | Cne => negb (NPeano.Nat.eqb n1 n2)
+                           | Cle => NPeano.Nat.leb n1 n2 
+                           | Cgt => negb (NPeano.Nat.leb n1 n2)
+                       end
+              in
+              if t  
+              then
+                dyncheck (mk (c s) (pc s +1 + ofs) stk  (str s) )
+              else
+                dyncheck (mk (c s) (pc s +1) stk  (str s) )
+             
+          end
+        | _ => None
+      end.
+  End t.
+(*             
+  Inductive transition (C: code): machine_state -> machine_state -> Prop :=
+  | trans_const: forall pc stk s n,
+                   code_at C pc = Some(Iconst n) ->
+                   transition C (pc, stk, s) (pc + 1, n :: stk, s)
+  | trans_var: forall pc stk s x,
+                 code_at C pc = Some(Ivar x) ->
+                 transition C (pc, stk, s) (pc + 1, s x :: stk, s)
+  | trans_setvar: forall pc stk s x n,
+                    code_at C pc = Some(Isetvar x) ->
+                    transition C (pc, n :: stk, s) (pc + 1, stk, update s x n)
+  | trans_add: forall pc stk s n1 n2,
+                 code_at C pc = Some(Iadd) ->
+                 transition C (pc, n2 :: n1 :: stk, s) (pc + 1, (n1 + n2) :: stk, s)
+  | trans_sub: forall pc stk s n1 n2,
+                 code_at C pc = Some(Isub) ->
+      transition C (pc, n2 :: n1 :: stk, s) (pc + 1, (n1 - n2) :: stk, s)
+  | trans_mul: forall pc stk s n1 n2,
+                 code_at C pc = Some(Imul) ->
+                 transition C (pc, n2 :: n1 :: stk, s) (pc + 1, (n1 * n2) :: stk, s)
+
+  | trans_branch_forward: forall pc stk s ofs pc',
+                            code_at C pc = Some(Ibranch_forward ofs) ->
+                            pc' = pc + 1 + ofs ->
+                            transition C (pc, stk, s) (pc', stk, s)
+  | trans_branch_backward: forall pc stk s ofs pc',
+                             code_at C pc = Some(Ibranch_backward ofs) ->
+                             pc' = pc + 1 - ofs ->
+                             transition C (pc, stk, s) (pc', stk, s)
+  | trans_beq: forall pc stk s ofs n1 n2 pc',
+                 code_at C pc = Some(Ibeq ofs) ->
+                 pc' = (if beq_nat n1 n2 then pc + 1 + ofs else pc + 1) ->
+                 transition C (pc, n2 :: n1 :: stk, s) (pc', stk, s)
+  | trans_bne: forall pc stk s ofs n1 n2 pc',
+                 code_at C pc = Some(Ibne ofs) ->
+                 pc' = (if beq_nat n1 n2 then pc + 1 else pc + 1 + ofs) ->
+                 transition C (pc, n2 :: n1 :: stk, s) (pc', stk, s)
+  | trans_ble: forall pc stk s ofs n1 n2 pc',
+                 code_at C pc = Some(Ible ofs) ->
+                 pc' = (if Nat.leb n1 n2 then pc + 1 + ofs else pc + 1) ->
+                 transition C (pc, n2 :: n1 :: stk, s) (pc', stk, s)
+  | trans_bgt: forall pc stk s ofs n1 n2 pc',
+                 code_at C pc = Some(Ibgt ofs) ->
+                 pc' = (if Nat.leb n1 n2 then pc + 1 else pc + 1 + ofs) ->
+                 transition C (pc, n2 :: n1 :: stk, s) (pc', stk, s).
+*)
+
+End Spec. 
+
+
+Module Circuit. 
 Section t. 
   Variable size : nat.
-  (* We use the following ocaml type as a reference, and give assign
+  (** We use the following ocaml type as a reference, and give assign
   opcodes to instructions accordingly
 
   type instr = 
@@ -44,30 +207,27 @@ Section t.
   Open Scope list_scope. 
   Definition INSTR := Ttuple (OPCODE :: VAL :: nil). 
   
-  (* type env =
-  {
-    reg : int array; 
-    stack   : int array; 
-    mutable sp : int;
-    code: instr array;
-    mutable pc  : int;     
-  }
+  (*
+      c   : code;      
+      pc : nat;
+      stk : stack;
+      str : store
    *)
   Definition Phi : state := 
     [
-      Tregfile n VAL;         (* the registers *)
+      Tregfile n INSTR;       (* the code *)
+      Treg VAL;                  (* the program counter *)
       Tregfile n VAL;         (* the stack *)
       Treg VAL;                 (* the stack pointer *)
-      Tregfile n INSTR;       (* the code *)
-      Treg VAL                  (* the program counter *)
+      Tregfile n VAL         (* the registers *)     
     ]. 
   
   Ltac set_env := 
-    set (REGS  := var_0 : var Phi (Tregfile n VAL));
-    set (STACK := var_S (var_0) : var Phi (Tregfile n VAL));
-    set (SP    := var_S (var_S (var_0)) : var Phi (Treg VAL));
-    set (CODE  := var_S (var_S (var_S (var_0))) : var Phi (Tregfile n INSTR));
-    set (PC    := var_S (var_S (var_S (var_S (var_0)))) : var Phi (Treg VAL)).
+    set (CODE  := (var_0) : var Phi (Tregfile n INSTR));
+    set (PC    := var_S (var_0) : var Phi (Treg VAL));
+    set (STACK := var_S (var_S (var_0)) : var Phi (Tregfile n VAL));
+    set (SP    := var_S (var_S (var_S (var_0))) : var Phi (Treg VAL));
+    set (REGS  := var_S (var_S (var_S (var_S (var_0)))) : var Phi (Tregfile n INSTR)).
     
   Definition opcode {V} (I : expr V INSTR) : expr V OPCODE. 
     eapply Enth. 2: apply I. apply var_0.  
@@ -78,18 +238,18 @@ Section t.
   Defined. 
   
   Open Scope action_scope. 
-  Notation "x \oplus y" := (OrElse _ _ _ x y) (at level 50, left associativity). 
+  Notation "x \oplus y" := (OrElse _ _ _ x y) (at level 51, right associativity). 
 
   Section code. 
     (* We parametrise the following code by the variable parameter of the PHOAS representation.   *)
     Variable V : type -> Type. 
-   
-    Let REGS  := var_0 : var Phi (Tregfile n VAL).
-    Let STACK := var_S (var_0) : var Phi (Tregfile n VAL).
-    Let SP    := var_S (var_S (var_0)) : var Phi (Treg VAL). 
-    Let CODE  := var_S (var_S (var_S (var_0))) : var Phi (Tregfile n INSTR).
-    Let PC    := var_S (var_S (var_S (var_S (var_0)))) : var Phi (Treg VAL).
-   
+
+    Definition CODE  := (var_0) : var Phi (Tregfile n INSTR).
+    Definition PC    := var_S (var_0) : var Phi (Treg VAL).
+    Definition STACK := var_S (var_S (var_0)) : var Phi (Tregfile n VAL).
+    Definition SP    := var_S (var_S (var_S (var_0))) : var Phi (Treg VAL).
+    Definition REGS  := var_S (var_S (var_S (var_S (var_0)))) : var Phi (Tregfile n VAL).
+    
     Definition push i : action Phi V Tunit :=
       (do sp <- ! SP;       
        do _ <- write STACK [: sp <- i];             
@@ -103,39 +263,28 @@ Section t.
       ret x. 
 
  
-    Definition Iconst : action Phi V Tunit := (
-      do pc <- ! PC; 
-      do i <- read CODE [: pc ]; 
-      WHEN (opcode i = (#i 0)); 
+    Definition Iconst  (pc: expr V VAL) (i : expr V INSTR) : action Phi V Tunit :=(
       do _ <- push (val i);
       PC ::= pc + #i 1              
     )%action.
-
-    Definition Ivar : action Phi V Tunit := 
+    
+    
+    Definition Ivar (pc: expr V VAL) (i : expr V INSTR) : action Phi V Tunit := 
       (
-        do pc <- ! PC; 
-        do i <- read CODE [: pc ]; 
-        WHEN (opcode i = (#i 1)); 
         do r <- read REGS [: val i];
         do _ <- push r;
         PC ::= pc + #i 1              
       )%action.
     
-    Definition Isetvar : action Phi V Tunit := 
+    Definition Isetvar (pc: expr V VAL) (i : expr V INSTR) : action Phi V Tunit := 
       (
-        do pc <- ! PC; 
-        do i <- read CODE [: pc ]; 
-        WHEN (opcode i = (#i 2)); 
         do v <- pop; 
         do _ <- write REGS [: val i <- v];
         PC ::= pc + #i 1              
       )%action.
      
-      Definition Iadd : action Phi V Tunit := 
+      Definition Iadd(pc: expr V VAL) (i : expr V INSTR) : action Phi V Tunit :=
       (
-        do pc <- ! PC; 
-        do i <- read CODE [: pc ]; 
-        WHEN (opcode i = (#i 3)); 
         do sp <- ! SP;       
         do n2 <- read STACK [: sp - #i 1];
         do n1 <- read STACK [: sp - #i 2];
@@ -144,11 +293,8 @@ Section t.
         PC ::= pc + #i 1              
       )%action.
       
-      Definition Isub : action Phi V Tunit := 
+      Definition Isub (pc: expr V VAL) (i : expr V INSTR) : action Phi V Tunit :=
       (
-        do pc <- ! PC; 
-        do i <- read CODE [: pc ]; 
-        WHEN (opcode i = (#i 4)); 
         do sp <- ! SP;       
         do n2 <- read STACK [: sp - #i 1];
         do n1 <- read STACK [: sp - #i 2];
@@ -157,27 +303,20 @@ Section t.
         PC ::= pc + #i 1              
       )%action.
       
-      Definition Ibranch_forward : action Phi V Tunit := 
+      Definition Ibranch_forward (pc: expr V VAL) (i : expr V INSTR) : action Phi V Tunit :=
       (
-        do pc <- ! PC; 
-        do i <- read CODE [: pc ]; 
-        WHEN (opcode i = (#i 5)); 
         PC ::= pc + #i 1 + (val i)              
       )%action.
-
-      Definition Ibranch_backward : action Phi V Tunit := 
+      
+      
+      
+      Definition Ibranch_backward (pc: expr V VAL) (i : expr V INSTR) : action Phi V Tunit :=
       (
-        do pc <- ! PC; 
-        do i <- read CODE [: pc ]; 
-        WHEN (opcode i = (#i 6)); 
         PC ::= pc + #i 1 - (val i)              
       )%action.      
       
-      Definition Ibranch_cond code cond : action Phi V Tunit := 
+      Definition Ibranch_cond cond (pc: expr V VAL) (i : expr V INSTR) : action Phi V Tunit :=
         (
-          do pc <- ! PC; 
-          do i <- read CODE [: pc ]; 
-          WHEN (opcode i = (#i code)); 
           do sp <- ! SP;       
           do n2 <- read STACK [: sp - #i 1];
           do n1 <- read STACK [: sp - #i 2];
@@ -187,47 +326,570 @@ Section t.
              \oplus (PC ::= pc + #i 1))
       )%action.      
 
-      Definition Ibeq: action Phi V Tunit := 
-        Ibranch_cond 7 (fun n1 n2 => n1 = n2)%expr. 
+      Definition Ibeq := 
+        Ibranch_cond (fun n1 n2 => n1 = n2)%expr. 
 
-      Definition Ibne: action Phi V Tunit := 
-        Ibranch_cond 8 (fun n1 n2 => n1 <> n2)%expr. 
+      Definition Ibne := 
+        Ibranch_cond (fun n1 n2 => n1 <> n2)%expr. 
       
-      Definition Ible: action Phi V Tunit := 
-        Ibranch_cond 9 (fun n1 n2 => n1 <= n2)%expr. 
+      Definition Ible := 
+        Ibranch_cond (fun n1 n2 => n1 <= n2)%expr. 
 
-      Definition Ibgt: action Phi V Tunit := 
-        Ibranch_cond 10 (fun n1 n2 => n2 < n1)%expr. 
+      Definition Ibgt := 
+        Ibranch_cond (fun n1 n2 => n2 < n1)%expr. 
       
-      Definition Ihalt: action Phi V Tbool := 
-        do pc <- ! PC; 
-        do i <- read CODE [: pc ]; 
+      Definition Ihalt (pc: expr V VAL) (i : expr V INSTR) : action Phi V B :=
         WHEN (opcode i = (#i 11)); 
         ret #b true.
       
-      (*
-  type instr = 
-  | Iconst of int 			(* push integer on stack *)
-  | Ivar   of reg 			(* push register on stack *)
-  | Isetvar of reg 			(* pop an integer into a register *)
-  | Iadd 					(* pop n2, pop n1, push back n1 + n2 *)
-  | Isub 					(* pop n2, pop n1, push back n1 - n2 *)
-  | Ibranch_forward of int 		(* move pc to pc + 1 + ofs *)
-  | Ibranch_backward of int 		(* move pc to pc + 1 - ofs *)
-  | Ibeq of int 				(* pop n2, pop n1, skips ofs forward if n1 = n2 *)
-  | Ibne of int 				(* pop n2, pop n1, skips ofs forward if n1 <> n2 *)
-  | Ible of int 				(* pop n2, pop n1, skips ofs forward if n1 <= n2 *)
-  | Ibgt of int 				(* pop n2, pop n1, skips ofs forward if n1 > n2 *)
-  | Ihalt
+      Definition code_at {T} f : action Phi V T:=
+        do pc <- ! PC;
+        do i  <- read CODE [: pc];
+        f pc i.
+      
+      Fixpoint case {S T} (x : expr V S) (l : list (expr V S * action Phi V T)) default :=
+        match l with 
+          | nil => default
+          | (c,a) :: q => 
+            (WHEN (x = c); a) 
+              \oplus case x q default
+        end. 
 
-       *)
-
+      Require Import ZArith. 
+      Definition mk_val {n} v : expr V (W n) := (#i (Z.of_nat v)).
+                              
       Definition code :=
-        (do _ <- (Iconst \oplus Ivar \oplus Isetvar \oplus Iadd \oplus Isub \oplus Ibranch_forward \oplus Ibranch_backward \oplus Ibeq \oplus Ible \oplus Ibgt); ret (#b false)) \oplus Ihalt.
+        code_at (fun pc i =>
+                   case (opcode i)
+                        ([
+                            (mk_val 0, Iconst pc i);
+                            (mk_val 1, Ivar   pc i);
+                            (mk_val 2, Isetvar pc i);
+                            (mk_val 3, Iadd pc i);
+                            (mk_val 4, Isub pc i);
+                            (mk_val 5, Ibranch_forward pc i);
+                            (mk_val 6, Ibranch_backward pc i);
+                            (mk_val 7, Ibeq pc i);
+                            (mk_val 8, Ibne pc i);
+                            (mk_val 9, Ible pc i);
+                            (mk_val 10, Ibgt pc i)
+                        ])
+                        ret (# Ctt )) .
   End code. 
   Definition Code := fun V => code V.  
-End t. 
+  Definition Next m := Front.Next _ m (Code).
+End t.
+End Circuit.
 
+Section t. 
+  Variable n : nat. 
+
+  Notation V := eval_type. 
+  
+  Definition step  {Phi t} (A : action Phi eval_type t) st : 
+    option (eval_state Phi) :=    
+    match Sem.eval_action  A st (Diff.init Phi)  with
+      | Some p => Some (Diff.apply Phi (snd p) st)
+      | None => None
+    end. 
+  Require Import ZArith DList. 
+  Definition mk_val v : eval_type (W n) := Word.repr n (Z.of_nat v).
+
+  Notation "x =%= y" := (mk_val x = y) (at level 80).
+  
+  Notation c  m2 := (DList.DList.get (Circuit.CODE n) m2).    
+  Notation pc m2 := (DList.DList.get (Circuit.PC n) m2).    
+  Notation stk m2 := (DList.DList.get (Circuit.STACK n) m2).
+  Notation sp m2 := (DList.DList.get (Circuit.SP n) m2).
+  (* 
+    Definition CODE  := (var_0) : var Phi (Tregfile n INSTR).
+    Definition PC    := var_S (var_0) : var Phi (Treg VAL).
+    Definition STACK := var_S (var_S (var_0)) : var Phi (Tregfile n VAL).
+    Definition SP    := var_S (var_S (var_S (var_0))) : var Phi (Treg VAL).
+    Definition REGS  := var_S (var_S (var_S (var_S (var_0)))) : var Phi (Tregfile n VAL).
+   *)
+
+  Eval compute in eval_type (Circuit.INSTR 3).
+  Require Import ZArith. 
+
+  Definition cast_instr op val : eval_type (Circuit.INSTR n) :=
+    (Word.repr _ (Z.of_nat op), (Word.repr _ (Z.of_nat val) , tt)).
+  Definition mk_instr (i : Spec.instruction) : eval_type (Circuit.INSTR n) :=
+    match i with
+      | Spec.Iconst x =>  cast_instr 0 x 
+      | Spec.Ivar x =>    cast_instr 1 x
+      | Spec.Isetvar x => cast_instr 2 x
+      | Spec.Iadd =>      cast_instr 3 0
+      | Spec.Isub =>      cast_instr 4 0
+      | Spec.Ibranch_forward ofs => cast_instr 5 ofs
+      | Spec.Ibranch_backward ofs => cast_instr 6 ofs
+      | Spec.Ibranch_cond Spec.Ceq ofs =>             cast_instr 7 ofs
+      | Spec.Ibranch_cond Spec.Cne ofs =>             cast_instr 8 ofs
+      | Spec.Ibranch_cond Spec.Cle ofs =>             cast_instr 9 ofs
+      | Spec.Ibranch_cond Spec.Cgt ofs =>             cast_instr 10 ofs
+      | Spec.Ihalt =>                cast_instr 11 0
+    end.
+
+  (** The property that states that the code on both machines are compatible  *)
+  Definition R_code (m1 : Spec.machine) (m2 : eval_state (Circuit.Phi n)) :  Prop :=
+    forall p, p < n -> 
+         match Spec.code_at (Spec.c m1) p with 
+           | None => False
+           | Some i => mk_instr i = Regfile.get (c m2) (mk_val p)
+         end.
+
+  (** We define what it means for stacks to be compatible *)
+  Definition R_stk l v := 
+    forall i i', i < List.length l ->  
+         i =%= i' ->
+         Regfile.get v i' = mk_val (List.nth i (List.rev l) 0).
+  
+  (** The invariant that relates the execution of the machines  *)
+  Record R (m1 : Spec.machine) (m2 : eval_state (Circuit.Phi n)) :  Prop := 
+    {
+      Rpc1 : Spec.pc m1 =%= pc m2;
+      Rpc2 : Spec.pc m1 < n;
+      Rstk : R_stk (Spec.stk m1) (stk m2);
+      Rsp : List.length (Spec.stk m1) =%= sp m2
+    }.
+
+  Notation "x == y" := (R x y) (at level 80).
+
+  Lemma step_code_at {T} m1 m2 (f : expr V (W n) -> expr V (Circuit.INSTR n) -> 
+                                  action (Circuit.Phi n) V T):          
+    R_code m1 m2 ->
+    m1 == m2 -> 
+    step (Circuit.code_at _ _ f)%action m2
+    = do i <- Spec.code_at (Spec.c m1) (Spec.pc m1);
+    step (f (Evar (mk_val (Spec.pc m1)))%expr (Evar (mk_instr i))) m2.
+  Proof. 
+    intros Hcode H.
+    unfold Circuit.code_at. 
+    unfold step at 1. Opaque DList.DList.get. Opaque Diff.apply.   
+    simpl. unfold Sem.Dyn.Bind.
+    rewrite (Rpc1 _ _ H).
+    refine (let H := Hcode (Spec.pc m1) (Rpc2 _ _ H) in _).     rewrite (Rpc1 _ _ H) in H0.
+    destruct (Spec.code_at (Spec.c m1) (Spec.pc m1)) eqn:?. simpl. rewrite H0. reflexivity. 
+    tauto. 
+  Qed.
+  
+  Add  Ring wring : (Word.ring n).
+    
+  Lemma repr_add m x y: Word.repr m (x + y) = Word.add (Word.repr m x) (Word.repr m y).
+    apply Word.unsigned_inj. simpl. 
+    rewrite Zplus_mod. reflexivity.
+  Qed. 
+
+  Lemma repr_sub m (x y : Z) : Word.repr m (x - y) = Word.sub (Word.repr m x) (Word.repr m y).
+  Proof.
+    apply Word.unsigned_inj; simpl.
+    rewrite Zminus_mod. reflexivity. 
+  Qed. 
+
+  Lemma Rval_succ : forall x, x + 1 =%= Word.add (mk_val x) (Cword 1%Z).
+  Proof. 
+    intros. 
+    unfold mk_val. rewrite plus_comm. rewrite Nat2Z.inj_succ.   rewrite <- Z.add_1_l. rewrite repr_add. unfold Cword. simpl. ring. 
+  Qed. 
+
+  Lemma Rval_add : forall x y, x + y =%= Word.add (mk_val x) (mk_val y).
+  Proof. 
+    intros. 
+    unfold mk_val. rewrite Nat2Z.inj_add. rewrite repr_add. reflexivity. 
+  Qed. 
+
+  Lemma Rval_sub : forall x y, y <= x -> x - y =%= Word.sub (mk_val x) (mk_val y%Z).
+  Proof.
+    intros. 
+    unfold mk_val. rewrite Nat2Z.inj_sub by omega. 
+    apply repr_sub. 
+  Qed. 
+
+
+  Lemma Rval_add_morphism : forall x1 y1 x2 y2, x1 =%= x2 -> y1 =%= y2 -> x1 + y1 =%= Word.add x2 y2. 
+  Proof. 
+    intros. rewrite <- H, <- H0. apply Rval_add. 
+  Qed. 
+  
+  Lemma Rval_sub_morphism : forall x1 y1 x2 y2, x1 =%= x2 -> y1 =%= y2 -> 
+                                                   y1 <= x1 -> x1 - y1 =%= Word.sub x2 y2. 
+  Proof. 
+    intros. 
+    rewrite <- H, <- H0. 
+    apply Rval_sub. omega. 
+  Qed. 
+
+  Lemma Rval_length_1 {A} (l: list A) hd tl x: 
+    l = hd :: tl ->
+    List.length l  =%= x ->
+    List.length tl =%= Word.sub x (Cword 1%Z).
+  Proof. 
+    intros. 
+    replace (List.length tl) with (List.length l - 1) by (rewrite H; simpl; try omega).  
+    rewrite <- H0. apply Rval_sub_morphism; auto. rewrite H. simpl; omega. 
+  Qed. 
+  Lemma Rval_length_2 {A} (l: list A) hd1 hd2 tl x: 
+    l = hd1 :: hd2 :: tl ->
+    List.length l  =%= x ->
+    List.length tl =%= Word.sub x (Cword 2%Z).
+  Proof. 
+    intros. 
+    replace (List.length tl) with (List.length l - 2) by (rewrite H; simpl; try omega).  
+    rewrite <- H0. apply Rval_sub_morphism; auto. rewrite H. simpl; omega. 
+  Qed. 
+  
+  (** We use the [val] hint db for theorems that deal with the Rval relation *)
+  Hint Resolve Rval_succ Rval_add Rval_sub Rval_add_morphism Rval_sub_morphism : val. 
+  Hint Resolve Rval_length_1 Rval_length_2 : val. 
+  
+  Lemma gso {size X} (v : Regfile.T size X) i j x: 
+    i <> j -> 
+    Regfile.get (Regfile.set v i x) j = Regfile.get v j.
+  Proof. 
+  Admitted. 
+  
+  Lemma gss {size X} (v : Regfile.T size X) i j x: 
+    i = j -> 
+    Regfile.get (Regfile.set v i x) j = x.
+  Proof. 
+  Admitted. 
+
+  Fixpoint case {A B} (eq : A -> A -> bool) e (l: list (A *B)) default :=
+    match l with 
+      | nil => default
+      | (t,v) :: q => if eq e t then v else case eq e q default
+      end.
+  
+    
+  Lemma step_case {S T k} (e: expr V S) l (default : action _ V T): 
+    step (Circuit.case k V e l default) =
+    step (case (fun x y => type_eq _ (eval_expr _ x) (eval_expr _ y)) e l default).
+  Proof. 
+  Admitted. 
+  
+  (** pushing elements on the stack preserves the stk part of the invariant *)
+  Lemma push_correct_stk stk1 stk2 x1 x2 p: x1 =%= x2 -> 
+                                      R_stk stk1 stk2  ->
+                                      p = mk_val (List.length stk1) ->
+                                      R_stk (x1 :: stk1) (Regfile.set (stk2) p x2).
+  Proof. 
+    unfold R_stk; simpl. intros Hx H Hp i i' Hi Hi'. rewrite <- Hi'. clear Hi'. 
+    assert (Hi' : i < List.length stk1 \/ i = (List.length stk1)) by omega; clear Hi.
+    destruct Hi' as [Hi | Hi]. 
+    * rewrite gso. rewrite List.app_nth1 by (rewrite List.rev_length;auto).      
+      apply H;auto. 
+      simpl in *. rewrite Hp. clear - Hi. admit. 
+    * rewrite List.app_nth2 by (rewrite List.rev_length;omega). 
+      rewrite Hi. rewrite List.rev_length. rewrite minus_diag. simpl. 
+      rewrite gss.  auto. 
+      simpl in *.  rewrite Hp. reflexivity. 
+  Qed.  
+  
+  Hint Extern 4  (_ < _) => rewrite <- NPeano.Nat.ltb_lt. 
+  (** pushing elements on the stack preserves the stack pointer part of the invariant  *)
+  Lemma push_correct_sp m1 m2 :
+    m1 == m2 -> 
+    S (Datatypes.length (Spec.stk m1)) =%=
+      Word.add (DList.hd (DList.tl (DList.tl (DList.tl m2)))) (Cword 1%Z).
+  Proof. 
+    destruct 1 as [_ _ _ H].
+    Transparent DList.get. simpl in *. Opaque DList.get.
+    rewrite <- H. rewrite <- NPeano.Nat.add_1_r. apply Rval_succ.        
+  Qed.   
+  Hint Resolve push_correct_sp.
+
+  Lemma pop_correct_stk hd tl v : R_stk (hd :: tl) (v) -> 
+                                      R_stk (tl) (v).
+  Proof.
+    unfold R_stk; simpl. intros. 
+    rewrite (H i); auto. 
+    rewrite List.app_nth1 by (rewrite List.rev_length; omega). reflexivity. 
+  Qed.
+  
+  Lemma pop_correct_sp m1 m2 hd tl k : m1 == m2 -> 
+                                     Spec.stk m1 = hd :: tl -> 
+                                     k = Datatypes.length tl -> 
+                                     k =%= Word.sub (DList.hd (DList.tl (DList.tl (DList.tl m2)))) (Cword 1%Z).
+  Proof. 
+    intros. unfold Cword. 
+    replace k with (List.length (Spec.stk m1) - 1). apply Rval_sub_morphism. 
+    destruct H; simpl in *; auto. 
+    reflexivity. 
+    rewrite H0; simpl; omega. 
+    rewrite H0. simpl. omega. 
+  Qed.
+  
+  Hint Resolve pop_correct_sp.
+
+
+  Lemma pop2_correct_sp m1 m2 hd1 hd2 tl k : m1 == m2 -> 
+                                        Spec.stk m1 = hd1 :: hd2 :: tl -> 
+                                        k = Datatypes.length tl -> 
+                                        k =%= Word.sub (DList.hd (DList.tl (DList.tl (DList.tl m2)))) (Cword 2%Z).
+  Proof. 
+    intros. unfold Cword. 
+    replace k with (List.length (Spec.stk m1) - 2). apply Rval_sub_morphism. 
+    destruct H; simpl in *; auto. 
+    reflexivity. 
+    rewrite H0; simpl; omega. 
+    rewrite H0. simpl. omega. 
+  Qed.
+  
+  Hint Resolve pop2_correct_sp.
+
+  Definition branch_cond_eval cond n1 n2 :=
+    match cond with
+      | Spec.Ceq => NPeano.Nat.eqb n1 n2
+      | Spec.Cne => negb (NPeano.Nat.eqb n1 n2)
+      | Spec.Cle => NPeano.Nat.leb n1 n2
+      | Spec.Cgt => negb (NPeano.Nat.leb n1 n2)
+    end.
+  
+  Require Import Consider. 
+
+  Ltac list_length_tac :=
+      repeat 
+        match goal with 
+            |- context [List.length (List.rev _)] => rewrite List.rev_length
+          | |- context [List.length (List.app _ _)] => rewrite List.app_length
+          | H : ?l = _ |- context [List.length ?l] => rewrite H
+        end; simpl; omega.
+  
+  Hint Extern 4  (_ < _) => list_length_tac. 
+  Hint Extern 4  (_ <= _) => list_length_tac. 
+  Hint Extern 4  (_ > _) => list_length_tac. 
+  Hint Extern 4  (_ >= _) => list_length_tac. 
+
+      
+  Transparent Diff.apply. Transparent Diff.add. Transparent Diff.init. 
+  Transparent DList.get. 
+  
+  Lemma branch_cond_correct m1 m2 (Hcode : R_code m1 m2) (H : m1 == m2) m1' 
+        (Hm1: Spec.step n m1 = Some m1') 
+        test
+        cond ofs
+        (Hi : Spec.code_at (Spec.c m1) (Spec.pc m1) = Some (Spec.Ibranch_cond cond ofs))
+        (Hcond : forall x1 y1 x2 y2, 
+              x1 =%= x2 -> 
+              y1 =%= y2 ->
+              eval_expr B (test (Evar x2) (Evar y2)) = branch_cond_eval cond x1 y1)
+  : 
+    match step (Circuit.Ibranch_cond n V test (Evar (mk_val (Spec.pc m1))) (Evar (mk_instr (Spec.Ibranch_cond cond ofs)))) m2 with 
+      | None => False
+      | Some m2' => m1' == m2'
+    end.      
+  Proof.
+    unfold Spec.step in Hm1; rewrite Hi in Hm1; simpl in Hm1. 
+    destruct (Spec.stk m1) as [ | n2 [| n1 s]] eqn: Hs; try discriminate. 
+    unfold step. simpl. unfold Sem.Dyn.Bind. unfold Sem.Dyn.OrElse. 
+    rewrite (Hcond n1 n2). 
+    destruct cond; simpl in *. 
+    - consider (NPeano.Nat.eqb n1 n2); intros Hn Hm.
+      unfold Spec.dyncheck in Hm; simpl in Hm;
+      consider (NPeano.Nat.ltb (Spec.pc m1 + 1 + ofs) n); intros Hofs Hm; try discriminate;
+      inject Hm; simpl.
+      constructor; simpl; eauto with *.  
+      destruct H; simpl in *; eauto. 
+      eapply (pop_correct_stk n2). 
+      eapply (pop_correct_stk n2). rewrite <- Hs. eauto. 
+
+      unfold Spec.dyncheck in Hm; simpl in Hm;
+      consider (NPeano.Nat.ltb (Spec.pc m1 + 1 ) n); intros Hofs Hm; try discriminate;
+      inject Hm; simpl.
+      constructor; simpl; eauto with *.  
+      destruct H; simpl in *; eauto. 
+      eapply (pop_correct_stk n1). 
+      eapply (pop_correct_stk n2). rewrite <- Hs. eauto. 
+    - consider (NPeano.Nat.eqb n1 n2); intros Hn Hm.
+      unfold Spec.dyncheck in Hm; simpl in Hm;
+      consider (NPeano.Nat.ltb (Spec.pc m1 + 1) n); intros Hofs Hm; try discriminate;
+      inject Hm; simpl.
+      constructor; simpl; eauto with *.  
+      destruct H; simpl in *; eauto. 
+      eapply (pop_correct_stk n2). 
+      eapply (pop_correct_stk n2). rewrite <- Hs. eauto. 
+
+      unfold Spec.dyncheck in Hm; simpl in Hm;
+      consider (NPeano.Nat.ltb (Spec.pc m1 + 1 +ofs) n); intros Hofs Hm; try discriminate;
+      inject Hm; simpl.
+      constructor; simpl; eauto with *.  
+      destruct H; simpl in *; eauto. 
+      eapply (pop_correct_stk n1). 
+      eapply (pop_correct_stk n2). rewrite <- Hs. eauto. 
+    - consider (NPeano.Nat.leb n1 n2); intros Hn Hm.
+      unfold Spec.dyncheck in Hm; simpl in Hm;
+      consider (NPeano.Nat.ltb (Spec.pc m1 + 1 + ofs) n); intros Hofs Hm; try discriminate;
+      inject Hm; simpl.
+      constructor; simpl; eauto with *.  
+      destruct H; simpl in *; eauto. 
+      eapply (pop_correct_stk n1). 
+      eapply (pop_correct_stk n2). rewrite <- Hs. eauto. 
+
+      unfold Spec.dyncheck in Hm; simpl in Hm;
+      consider (NPeano.Nat.ltb (Spec.pc m1 + 1) n); intros Hofs Hm; try discriminate;
+      inject Hm; simpl.
+      constructor; simpl; eauto with *.  
+      destruct H; simpl in *; eauto. 
+      eapply (pop_correct_stk n1). 
+      eapply (pop_correct_stk n2). rewrite <- Hs. eauto. 
+    - consider (NPeano.Nat.leb n1 n2); intros Hn Hm.
+      unfold Spec.dyncheck in Hm; simpl in Hm;
+      consider (NPeano.Nat.ltb (Spec.pc m1 + 1 ) n); intros Hofs Hm; try discriminate;
+      inject Hm; simpl.
+      constructor; simpl; eauto with *.  
+      destruct H; simpl in *; eauto. 
+      eapply (pop_correct_stk n1). 
+      eapply (pop_correct_stk n2). rewrite <- Hs. eauto. 
+
+      unfold Spec.dyncheck in Hm; simpl in Hm;
+      consider (NPeano.Nat.ltb (Spec.pc m1 + 1 + ofs) n); intros Hofs Hm; try discriminate;
+      inject Hm; simpl.
+      constructor; simpl; eauto with *.  
+      destruct H; simpl in *; eauto. 
+      eapply (pop_correct_stk n1). 
+      eapply (pop_correct_stk n2). rewrite <- Hs. eauto. 
+    - clear Hcond Hm1. 
+      destruct H. rewrite (Rstk0 (List.length (Spec.stk m1) - 2)); auto. 
+      rewrite Hs. simpl. rewrite List.app_nth1. rewrite List.app_nth2. 
+      rewrite List.rev_length. 
+      rewrite <- minus_n_O. rewrite minus_diag.  simpl. reflexivity. 
+      rewrite List.rev_length. omega.  simpl. 
+      auto. 
+      auto.
+      apply Rval_sub_morphism. apply Rsp0. reflexivity. 
+      auto. 
+    - clear Hcond Hm1. 
+      destruct H. rewrite (Rstk0 (List.length (Spec.stk m1) - 1)); auto. 
+      rewrite Hs. simpl. rewrite List.app_nth2. 
+      rewrite List.app_length.
+      rewrite List.rev_length. simpl List.length.  rewrite plus_comm. simpl plus. rewrite minus_diag. simpl. reflexivity. 
+      auto. 
+      apply Rval_sub_morphism. apply Rsp0. reflexivity.  auto. 
+      
+  Qed. 
+
+                          (****************)
+                          (* MAIN THEOREM *)
+                          (****************)
+  
+  Theorem circuit_correct m1 m2 (Hcode : R_code m1 m2) : 
+           m1 == m2 -> 
+    forall m1', 
+    Spec.step n m1 = Some m1' -> 
+    match step (Circuit.Code n V) m2 with 
+      | None => False
+      | Some m2' => m1' == m2'
+    end.
+  Proof.     
+    intros H m1' Hm1. 
+    unfold Next. unfold Circuit.Code, Circuit.code.  
+    erewrite step_code_at by eassumption.  Opaque Circuit.case.
+    intro_do i Hi.
+    rewrite step_case. 
+
+    2: (destruct H as [H1];
+        refine (let H := Hcode (Spec.pc m1) _ in _);
+        [admit |  rewrite Hi in H; tauto]). 
+    
+    
+  
+    destruct i; unfold case, type_eq;
+    repeat match goal with 
+             | |- context [Word.eqb ?x ?y] => replace (Word.eqb x y) with true by reflexivity
+             |  |- context [Word.eqb ?x ?y] => replace (Word.eqb x y) with false by reflexivity
+           end.
+    - (** Iconst *)
+      unfold Spec.step in Hm1; rewrite Hi in Hm1;simpl in Hm1; unfold Spec.dyncheck in Hm1; simpl in Hm1; match goal with | H : context [NPeano.Nat.ltb ?x ?y] |- _ => destruct (NPeano.Nat.ltb x y) eqn:? end; simpl in Hm1.  inject Hm1. 
+      simpl. Transparent DList.get. Transparent Diff.apply.       simpl. 
+      constructor; simpl.
+      + auto with val.
+      + auto. 
+      + intros. apply push_correct_stk; destruct H; simpl in *; auto. 
+      + auto. 
+      + discriminate. 
+    - (** Ivar *)
+      unfold Spec.step in Hm1; rewrite Hi in Hm1;simpl in Hm1; unfold Spec.dyncheck in Hm1; simpl in Hm1; match goal with | H : context [NPeano.Nat.ltb ?x ?y] |- _ => destruct (NPeano.Nat.ltb x y) eqn:? end; simpl in Hm1.  inject Hm1.  
+      constructor; simpl. 
+      + auto with val.  
+      + auto. 
+      + apply push_correct_stk. admit. destruct H; simpl in *; auto. destruct H; simpl in *; auto. 
+      + auto. 
+      + discriminate. 
+    - (** Isetvar *)                        
+      unfold Spec.step in Hm1; rewrite Hi in Hm1;simpl in Hm1; unfold Spec.dyncheck in Hm1; simpl in Hm1; match goal with | H : context [NPeano.Nat.ltb ?x ?y] |- _ => destruct (NPeano.Nat.ltb x y) eqn:? end; simpl in Hm1; destruct (Spec.stk m1) eqn:?; try discriminate. inject Hm1.  
+      simpl.  
+      constructor;simpl. 
+      + auto with val. 
+      + auto. 
+      + apply (pop_correct_stk n0 s) . rewrite <- Heqs. destruct H.  simpl in *; eauto. 
+      + eauto.           
+    - unfold Spec.step in Hm1; rewrite Hi in Hm1;simpl in Hm1; unfold Spec.dyncheck in Hm1; simpl in Hm1; match goal with | H : context [NPeano.Nat.ltb ?x ?y] |- _ => destruct (NPeano.Nat.ltb x y) eqn:? end; simpl in Hm1;  destruct (Spec.stk m1) as [ | a1 [ |a2 s]] eqn:?; try discriminate. inject Hm1.  
+      {
+        constructor; simpl.  
+        + auto with val. 
+        + auto. 
+        + intros. 
+          eapply push_correct_stk.
+          {apply Rval_add_morphism. destruct H. unfold R_stk in *. admit. admit. } 
+          eapply (pop_correct_stk a2). eapply (pop_correct_stk a1). 
+          rewrite <- Heqs. destruct H. simpl in *. eauto.
+          replace (List.length s) with (List.length (Spec.stk m1) - 2).
+          simpl. rewrite (Rval_sub _ 2). f_equal. destruct H; simpl in *; eauto. rewrite Heqs. simpl. omega. rewrite Heqs. simpl. omega. 
+        + eauto using  pop_correct_sp.   
+      }
+    - (** Isub *)
+      unfold Spec.step in Hm1; rewrite Hi in Hm1;simpl in Hm1; unfold Spec.dyncheck in Hm1; simpl in Hm1; match goal with | H : context [NPeano.Nat.ltb ?x ?y] |- _ => destruct (NPeano.Nat.ltb x y) eqn:? end; simpl in Hm1;  destruct (Spec.stk m1) as [ | a2 [ |a1 s]] eqn:?; try discriminate. inject Hm1.
+      {
+        constructor; simpl. 
+        + auto with val. 
+        + auto. 
+        + intros.  eapply push_correct_stk. admit. eapply (pop_correct_stk a1). eapply (pop_correct_stk a2). rewrite <- Heqs. destruct H; simpl in *; eauto. 
+          replace (List.length s) with (List.length (Spec.stk m1) - 2). 
+          simpl. rewrite (Rval_sub _ 2). f_equal. destruct H. simpl in *. eauto. rewrite Heqs. simpl. omega. rewrite Heqs. simpl. omega. 
+        + eauto using pop_correct_sp. 
+      }
+    -  (** Branch_forward *)
+      unfold Spec.step in Hm1; rewrite Hi in Hm1;simpl in Hm1; unfold Spec.dyncheck in Hm1; simpl in Hm1; match goal with | H : context [NPeano.Nat.ltb ?x ?y] |- _ => destruct (NPeano.Nat.ltb x y) eqn:? end; simpl in Hm1; try discriminate. inject Hm1.
+      {
+        constructor; simpl. 
+        + 
+          auto using Rval_add_morphism. 
+        + auto. 
+        + destruct H; simpl in *; auto. 
+        + destruct H; simpl in *; auto.       
+      }      
+    - 
+      unfold Spec.step in Hm1; rewrite Hi in Hm1;simpl in Hm1; unfold Spec.dyncheck in Hm1; simpl in Hm1.  
+      consider (NPeano.leb ofs (Spec.pc m1 + 1)); intros Hofs; try discriminate. 
+      consider (NPeano.Nat.ltb (Spec.pc m1 + 1 - ofs) n); intros Hofs'; try discriminate. 
+      intros Hm. inject Hm. 
+      simpl. 
+      {
+        constructor; simpl. 
+        + auto with val. 
+        + auto. 
+        + destruct H; simpl in *; auto. 
+        + destruct H; simpl in *; auto.       
+      } 
+    - destruct c; 
+      repeat match goal with 
+             | |- context [Word.eqb ?x ?y] => replace (Word.eqb x y) with true by reflexivity
+             |  |- context [Word.eqb ?x ?y] => replace (Word.eqb x y) with false by reflexivity
+           end;
+      apply branch_cond_correct; auto. 
+      + clear. intros. simpl. rewrite <- H, <- H0.
+        admit. 
+      + clear. intros. simpl. rewrite <- H, <- H0.
+        admit. 
+      + clear. intros. simpl. rewrite <- H, <- H0.
+        admit. 
+      + clear. intros. simpl. rewrite <- H, <- H0.
+        admit. 
+    - simpl. 
+      unfold Spec.step in Hm1; rewrite Hi in Hm1; simpl in Hm1; unfold Spec.dyncheck in Hm1; simpl in Hm1. discriminate. 
+  Qed.
+
+  Print Assumptions circuit_correct. 
 Require Compiler. 
 Require Import FirstOrder RTL Core. 
 
